thys/Transition_Systems_and_Automata/Basic/Sequence_LTL.thy
@@ -8,12 +8,14 @@ begin
 
   subsection \<open>Basics\<close>
 
-  text \<open>Avoid destroying the constant @{term holds} prematurely.\<close>
+  text \<open>Avoid destroying the constant @{const holds} prematurely.\<close>
   lemmas [simp del] = holds.simps holds_eq1 holds_eq2 not_holds_eq
 
+  lemma ev_smap[iff]: "ev P (smap f w) \<longleftrightarrow> ev (P \<circ> smap f) w" using ev_smap unfolding comp_apply by this
+  lemma alw_smap[iff]: "alw P (smap f w) \<longleftrightarrow> alw (P \<circ> smap f) w" using alw_smap unfolding comp_apply by this
   lemma holds_smap[iff]: "holds P (smap f w) \<longleftrightarrow> holds (P \<circ> f) w" unfolding holds.simps by simp
 
-  lemmas [iff] = ev_sconst alw_sconst ev_smap alw_smap hld_smap'
+  lemmas [iff] = ev_sconst alw_sconst hld_smap'
 
   lemmas [iff] = alw_ev_stl
   lemma alw_ev_sdrop[iff]: "alw (ev P) (sdrop n w) \<longleftrightarrow> alw (ev P) w"
